PalamedesTest/Examples/Simple/OneOfFour.lean
@@ -1,0 +1,6 @@
+import Palamedes.Synthesizer
+
+open Palamedes Palamedes.Gen Palamedes.Gen.CorrectGen
+
+def genSmall : Gen Nat := by
+  generator_search (fun a => a = 1 ∨ a = 2 ∨ a = 3 ∨ a = 4)
